theories/lang/races.v
@@ -31,24 +31,24 @@ Inductive next_access_head : expr → state → access_kind * order → loc → 
 Goal ∀ e1 e2 e3 σ, head_reducible (CAS e1 e2 e3) σ →
                    ∃ a l, next_access_head (CAS e1 e2 e3) σ a l.
 Proof.
-  intros ??? σ (?&?&?&?). inversion H; do 2 eexists;
+  intros ??? σ (?&?&?&?&?). inversion H; do 2 eexists;
     (eapply Access_cas_fail; done) || eapply Access_cas_suc; done.
 Qed.
 Goal ∀ o e σ, head_reducible (Read o e) σ →
               ∃ a l, next_access_head (Read o e) σ a l.
 Proof.
-  intros ?? σ (?&?&?&?). inversion H; do 2 eexists; eapply Access_read; done.
+  intros ?? σ (?&?&?&?&?). inversion H; do 2 eexists; eapply Access_read; done.
 Qed.
 Goal ∀ o e1 e2 σ, head_reducible (Write o e1 e2) σ →
               ∃ a l, next_access_head (Write o e1 e2) σ a l.
 Proof.
-  intros ??? σ (?&?&?&?). inversion H; do 2 eexists;
+  intros ??? σ (?&?&?&?&?). inversion H; do 2 eexists;
     eapply Access_write; try done; eexists; done.
 Qed.
 Goal ∀ e1 e2 σ, head_reducible (Free e1 e2) σ →
               ∃ a l, next_access_head (Free e1 e2) σ a l.
 Proof.
-  intros ?? σ (?&?&?&?). inversion H; do 2 eexists; eapply Access_free; done.
+  intros ?? σ (?&?&?&?&?). inversion H; do 2 eexists; eapply Access_free; done.
 Qed.
 
 Definition next_access_thread (e: expr) (σ : state)
@@ -80,7 +80,7 @@ Proof.
 Qed.
 
 Definition head_reduce_not_to_stuck (e : expr) (σ : state) :=
-  ∀ e' σ' efs, ectx_language.head_step e σ e' σ' efs → e' ≠ App (Lit $ LitInt 0) [].
+  ∀ κ e' σ' efs, ectx_language.head_step e σ κ e' σ' efs → e' ≠ App (Lit $ LitInt 0) [].
 
 Lemma next_access_head_reducible_state e σ a l :
   next_access_head e σ a l → head_reducible e σ →
@@ -93,7 +93,7 @@ Lemma next_access_head_reducible_state e σ a l :
   | (FreeAcc, _) => ∃ v ls, σ !! l = Some (ls, v)
   end.
 Proof.
-  intros Ha (e'&σ'&ef&Hstep) Hrednonstuck. destruct Ha; inv_head_step; eauto.
+  intros Ha (κ&e'&σ'&ef&Hstep) Hrednonstuck. destruct Ha; inv_head_step; eauto.
   - destruct n; first by eexists. exfalso. eapply Hrednonstuck; last done.
     by eapply CasStuckS.
   - exfalso. eapply Hrednonstuck; last done.
@@ -101,17 +101,17 @@ Proof.
   - match goal with H : ∀ m, _ |- _ => destruct (H i) as [_ [[]?]] end; eauto.
 Qed.
 
-Lemma next_access_head_Na1Ord_step e1 e2 ef σ1 σ2 a l :
+Lemma next_access_head_Na1Ord_step e1 e2 ef σ1 σ2 κ a l :
   next_access_head e1 σ1 (a, Na1Ord) l →
-  head_step e1 σ1 e2 σ2 ef →
+  head_step e1 σ1 κ e2 σ2 ef →
   next_access_head e2 σ2 (a, Na2Ord) l.
 Proof.
   intros Ha Hstep. inversion Ha; subst; clear Ha; inv_head_step; constructor; by rewrite to_of_val.
 Qed.
 
-Lemma next_access_head_Na1Ord_concurent_step e1 e1' e2 e'f σ σ' a1 a2 l :
+Lemma next_access_head_Na1Ord_concurent_step e1 e1' e2 e'f σ σ' κ a1 a2 l :
   next_access_head e1 σ (a1, Na1Ord) l →
-  head_step e1 σ e1' σ' e'f →
+  head_step e1 σ κ e1' σ' e'f →
   next_access_head e2 σ a2 l →
   next_access_head e2 σ' a2 l.
 Proof.
@@ -126,8 +126,8 @@ Proof.
     cut (is_Some (σ !! l)); last by eexists. rewrite -(elem_of_dom (D:=gset loc)). set_solver+.
 Qed.
 
-Lemma next_access_head_Free_concurent_step e1 e1' e2 e'f σ σ' o1 a2 l :
-  next_access_head e1 σ (FreeAcc, o1) l → head_step e1 σ e1' σ' e'f →
+Lemma next_access_head_Free_concurent_step e1 e1' e2 e'f σ σ' κ o1 a2 l :
+  next_access_head e1 σ (FreeAcc, o1) l → head_step e1 σ κ e1' σ' e'f →
   next_access_head e2 σ a2 l → head_reducible e2 σ' →
   False.
 Proof.
@@ -143,45 +143,45 @@ Proof.
       destruct l; intros [=?]. lia. }
   assert (FREE' : σ' !! l = None).
   { inversion Ha1; clear Ha1; inv_head_step. auto. }
-  destruct Hred2 as (e2'&σ''&ef&?).
+  destruct Hred2 as (κ'&e2'&σ''&ef&?).
   inversion Ha2; clear Ha2; inv_head_step.
   eapply (@is_Some_None (lock_state * val)). rewrite -FREE'. naive_solver.
 Qed.
 
-Lemma safe_step_not_reduce_to_stuck el σ K e e' σ' ef :
-  (∀ el' σ' e', rtc step (el, σ) (el', σ') →
+Lemma safe_step_not_reduce_to_stuck el σ K e e' σ' ef κ :
+  (∀ el' σ' e', rtc erased_step (el, σ) (el', σ') →
                 e' ∈ el' → to_val e' = None → reducible e' σ') →
-  fill K e ∈ el → head_step e σ e' σ' ef → head_reduce_not_to_stuck e' σ'.
+  fill K e ∈ el → head_step e σ κ e' σ' ef → head_reduce_not_to_stuck e' σ'.
 Proof.
-  intros Hsafe Hi Hstep e1 σ1 ? Hstep1 Hstuck.
+  intros Hsafe Hi Hstep κ1 e1 σ1 ? Hstep1 Hstuck.
   cut (reducible (fill K e1) σ1).
-  { subst. intros (?&?&?&?). by eapply stuck_irreducible. }
+  { subst. intros (?&?&?&?&?). by eapply stuck_irreducible. }
   destruct (elem_of_list_split _ _ Hi) as (?&?&->).
   eapply Hsafe; last by (apply: fill_not_val; subst).
   - eapply rtc_l, rtc_l, rtc_refl.
-    + econstructor. done. done. econstructor; done.
-    + econstructor. done. done. econstructor; done.
+    + eexists. econstructor. done. done. econstructor; done.
+    + eexists. econstructor. done. done. econstructor; done.
   - subst. set_solver+.
 Qed.
 
 (* TODO: Unify this and the above. *)
 Lemma safe_not_reduce_to_stuck el σ K e :
-  (∀ el' σ' e', rtc step (el, σ) (el', σ') →
+  (∀ el' σ' e', rtc erased_step (el, σ) (el', σ') →
                 e' ∈ el' → to_val e' = None → reducible e' σ') →
   fill K e ∈ el → head_reduce_not_to_stuck e σ.
 Proof.
-  intros Hsafe Hi e1 σ1 ? Hstep1 Hstuck.
+  intros Hsafe Hi κ e1 σ1 ? Hstep1 Hstuck.
   cut (reducible (fill K e1) σ1).
-  { subst. intros (?&?&?&?). by eapply stuck_irreducible. }
+  { subst. intros (?&?&?&?&?). by eapply stuck_irreducible. }
   destruct (elem_of_list_split _ _ Hi) as (?&?&->).
   eapply Hsafe; last by (apply: fill_not_val; subst).
   - eapply rtc_l, rtc_refl.
-    + econstructor. done. done. econstructor; done.
+    + eexists. econstructor. done. done. econstructor; done.
   - subst. set_solver+.
 Qed.
 
 Theorem safe_nonracing el σ :
-  (∀ el' σ' e', rtc step (el, σ) (el', σ') →
+  (∀ el' σ' e', rtc erased_step (el, σ) (el', σ') →
                 e' ∈ el' → to_val e' = None → reducible e' σ') →
   nonracing_threadpool el σ.
 Proof.
@@ -194,14 +194,14 @@ Proof.
   assert (Hnse1:head_reduce_not_to_stuck e1 σ).
   { eapply safe_not_reduce_to_stuck with (K:=K1); first done. set_solver+. }
   assert (Hσe1:=next_access_head_reducible_state _ _ _ _ Ha1 Hrede1 Hnse1).
-  destruct Hrede1 as (e1'&σ1'&ef1&Hstep1). clear Hnse1.
+  destruct Hrede1 as (κ1'&e1'&σ1'&ef1&Hstep1). clear Hnse1.
   assert (Ha1' : a1.2 = Na1Ord → next_access_head e1' σ1' (a1.1, Na2Ord) l).
   { intros. eapply next_access_head_Na1Ord_step, Hstep1.
     by destruct a1; simpl in *; subst. }
   assert (Hrtc_step1:
-    rtc step (t1 ++ fill K1 e1 :: t2 ++ fill K2 e2 :: t3, σ)
+    rtc erased_step (t1 ++ fill K1 e1 :: t2 ++ fill K2 e2 :: t3, σ)
         (t1 ++ fill K1 e1' :: t2 ++ fill K2 e2 :: t3 ++ ef1, σ1')).
-  { eapply rtc_l, rtc_refl. eapply step_atomic, Ectx_step, Hstep1; try  done.
+  { eapply rtc_l, rtc_refl. eexists. eapply step_atomic, Ectx_step, Hstep1; try  done.
     by rewrite -assoc. }
   assert (Hrede1: a1.2 = Na1Ord → head_reducible e1' σ1').
   { destruct a1 as [a1 []]=>// _.
@@ -218,14 +218,14 @@ Proof.
   assert (Hnse2:head_reduce_not_to_stuck e2 σ).
   { eapply safe_not_reduce_to_stuck with (K:=K2); first done. set_solver+. }
   assert (Hσe2:=next_access_head_reducible_state _ _ _ _ Ha2 Hrede2 Hnse2).
-  destruct Hrede2 as (e2'&σ2'&ef2&Hstep2).
+  destruct Hrede2 as (κ2'&e2'&σ2'&ef2&Hstep2).
   assert (Ha2' : a2.2 = Na1Ord → next_access_head e2' σ2' (a2.1, Na2Ord) l).
   { intros. eapply next_access_head_Na1Ord_step, Hstep2.
     by destruct a2; simpl in *; subst. }
   assert (Hrtc_step2:
-    rtc step (t1 ++ fill K1 e1 :: t2 ++ fill K2 e2 :: t3, σ)
+    rtc erased_step (t1 ++ fill K1 e1 :: t2 ++ fill K2 e2 :: t3, σ)
         (t1 ++ fill K1 e1 :: t2 ++ fill K2 e2' :: t3 ++ ef2, σ2')).
-  { eapply rtc_l, rtc_refl. rewrite app_comm_cons assoc.
+  { eapply rtc_l, rtc_refl. rewrite app_comm_cons assoc. eexists.
     eapply step_atomic, Ectx_step, Hstep2; try done. by rewrite -assoc. }
   assert (Hrede2: a2.2 = Na1Ord → head_reducible e2' σ2').
   { destruct a2 as [a2 []]=>// _.
@@ -280,7 +280,8 @@ Proof.
     end;
     try congruence.
 
-  clear e2' Hnse2' Hnse2_1 Hstep2 σ2' Hrtc_step2 Hrede2_1. destruct Hrede1_2 as (e2'&σ'&ef&?).
+  clear κ2' e2' Hnse2' Hnse2_1 Hstep2 σ2' Hrtc_step2 Hrede2_1.
+  destruct Hrede1_2 as (κ2'&e2'&σ'&ef&?).
   inv_head_step.
   match goal with
   | H : <[l:=_]> σ !! l = _ |- _ => by rewrite lookup_insert in H
@@ -289,7 +290,7 @@ Qed.
 
 Corollary adequate_nonracing e1 t2 σ1 σ2 φ :
   adequate NotStuck e1 σ1 φ →
-  rtc step ([e1], σ1) (t2, σ2) →
+  rtc erased_step ([e1], σ1) (t2, σ2) →
   nonracing_threadpool t2 σ2.
 Proof.
   intros [_ Had] Hrtc. apply safe_nonracing. intros el' σ' e' ?? He'.
